basic capture groups

parser/regex.dfy
@@ -1,4 +1,126 @@
 
+include "../libraries/src/Wrappers.dfy"
 module RegEx {
-    
+    import opened Wrappers
+    datatype RegexPiece = Char(value: char) | GroupStart(id: int) | GroupEnd(id: int) | Plus | Star | Optional | Alt | Concat
+    datatype Paren = Paren(natom: int, nalt: int)
+    function RegToChar(re: RegexPiece): char {
+        match re {
+            case Char(value) => value
+            case GroupStart(id) => '('
+            case GroupEnd(id) => ')'
+            case Alt => '|'
+            case Optional => '?'
+            case Plus => '+'
+            case Star => '*'
+            case Concat => '.'
+        }
+    }
+
+    method re2post(re: string) returns (res: Result<seq<RegexPiece>, string>) {
+        var buf := [];
+        var nalt := 0;
+        var natom := 0;
+        var groupid := 1;
+        var groups: seq<int> := [];
+        var parens: seq<Paren> :=[];
+        for i := 0 to |re| 
+
+        {
+            match re[i] {
+                case '(' => {
+                    if natom > 1 {
+                        natom := natom -1;
+                        buf := buf + [Concat];
+                    }
+                    parens := parens + [Paren(nalt, natom)];
+                    buf := buf + [GroupStart(groupid)];
+                    groups := groups + [groupid];
+                    groupid := groupid + 1;
+                    nalt := 0;
+                    natom := 0;
+                }
+                case '|' => {
+                    if natom == 0 {
+                        return Failure("Missing atom");
+                    }
+                    while natom > 0 {
+                        buf := buf + [Concat];
+                        natom := natom - 1;
+                    }
+                    nalt := nalt + 1;
+                }
+                case ')' => {
+                    if |parens| == 0 || |groups| == 0 || natom == 0 {
+                        return Failure("missing atom or paren");
+                    }
+                    while natom > 0 {
+                        buf := buf + [Concat];
+                        natom := natom - 1;
+                    }
+                    while nalt > 0 {
+                        buf := buf + [Alt];
+                        nalt := nalt - 1;
+                    }
+                    var next := parens[|parens|-1];
+                    nalt := next.nalt;
+                    natom := next.natom;
+                    parens := parens[0..|parens|-1];
+                    natom := natom + 1;
+                    buf := buf + [GroupEnd(groups[|groups|-1])];
+                    groups := groups[0..|groups|-1];
+                }
+                case '*' => {
+                    if natom == 0 {
+                        return Failure("Missing atom");
+                    }
+                    buf := buf + [Star];
+                }
+                case '+' => {
+                    if natom == 0 {
+                        return Failure("Missing atom");
+                    }
+                    buf := buf + [Plus];
+                }
+                case '?' => {
+                    if natom == 0 {
+                        return Failure("Missing atom");
+                    }
+                    buf := buf + [Optional];
+                }
+                case _ => {
+                    if natom > 1 {
+                        natom := natom -1;
+                        buf := buf + [Concat];
+                    }
+                    buf := buf + [Char(re[i])];
+                    natom := natom + 1;
+                }
+            }
+        }
+        if |parens| != 0 {
+            return Failure("Missing )");
+        }
+        while natom > 0 {
+            buf := buf + [Concat];
+            natom := natom - 1;
+        }
+        while nalt > 0 {
+            buf := buf + [Alt];
+            nalt := nalt - 1;
+        }
+        return Success(buf);
+    }
+
+    method Main() {
+        var test := re2post("a(a+be*)(c|(d)|f)g");
+        // var test := re2post("ac+de?(fg)*");
+        print test;
+        print "\n";
+        match test {
+            case Success(value) => print seq(|value|, i requires 0 <= i < |value| => RegToChar(value[i]));
+            case Failure(err) => print err;
+        }
+        
+    }
 }
